Revert "First attempt at views for hprops, and automatic equalities for delta through normalization" that I did not intend to push to the steel branch
This reverts commit b78bcbb5a62eab8690779bf2c53c7a0e8e3c11dd.

pulse/ulib/experimental/Steel.Memory.RST.fst
@@ -18,145 +18,34 @@ effect ST (a:Type) (pre:gst_pre) (post: (m0:mem -> Tot (gst_post' a (pre m0)))) 
   GST a
     (fun (p:gst_post a) (h:mem) -> pre h /\ (forall a h1. (pre h /\ post h a h1) ==> p a h1))
 
-(** TODO: Add a value_depends_only_on fp predicate. With this predicate,
-    we should be able to conclude that any predicate defined using only the views
-    is on fp_prop fp **)
-type view (a:Type) (fp:hprop) = (m:hheap fp) -> a
-
-(** An extension of hprops to include a view.
-    Note that the type of the view is not related to the fprop, and is completely up to the user.
-    For hprops for which we cannot defined a view, we thus could use unit.
-    TODO: This should have a better name. hprop_with_view?
-    **)
-noeq
-type viewable' = {
-    t:Type0;
-    fp:hprop;
-    sel:view t fp }
-
-(** Redefine an inductive for Star on top of hprops/viewables. This will allow us
-    to normalize by induction on the datatype **)
-noeq type viewable =
-   | VUnit: viewable' -> viewable
-   | VStar: viewable -> viewable -> viewable
-
-(** TODO: Could we go to a "flat" representation of tuples from t_of? **)
-let rec t_of (v:viewable) = match v with
-  | VUnit v -> v.t
-  | VStar v1 v2 -> (t_of v1 * t_of v2)
-
-let rec fp_of (v:viewable) = match v with
-  | VUnit v -> v.fp
-  | VStar v1 v2 -> (fp_of v1 `star` fp_of v2)
-
-let rec sel_of (v:viewable) (h:hheap (fp_of v)) : t_of v = match v with
-  | VUnit v -> v.sel h
-  | VStar v1 v2 ->
-    affine_star (fp_of v1) (fp_of v2) h;
-    (sel_of v1 h, sel_of v2 h)
-
-(** Completely incorrect, but used for test purposes. In the tests below, the left resource
-    will always be the leftmost starred hprop **)
-let rec incorrect_left_sel
-  (outer inner:viewable)
-  (delta:viewable)
-  (v:t_of outer)
-  : GTot (t_of inner)
-  = match outer with
-    | VUnit r -> assume (VUnit r == inner); v
-    | VStar r1 r2 ->
-      let (v1, v2) : t_of r1 * t_of r2 = v in incorrect_left_sel r1 inner delta v1
-
-(** Similar for right_sel **)
-let rec incorrect_right_sel
-  (outer:viewable{VStar? outer})
-  (inner delta:viewable)
-  (v:t_of outer)
-  : GTot (t_of delta)
-  = match outer with
-    | VStar (VUnit r1) r2 ->
-        let (v1, v2) : t_of (VUnit r1) * t_of r2 = v in
-        assume (r2 == delta);
-        v2
-    | VStar r1 r2 ->
-        let (v1, v2) : t_of r1 * t_of r2 = v in
-        admit();
-        incorrect_right_sel r1 inner delta v1, v2
-
-assume val can_be_split_into (outer inner delta:viewable) : prop
-
-(** AF: These functions should be the ones actually doing the rewriting in the end.
-    I think we can implement them using a variant of the canon_monoid tactic.
-    The postconditions are here for documentation purposes, we would probably need them
-    as lemmas to prove the correctness of frame
-    **)
-assume val left_sel
-  (outer inner:viewable)
-  (delta:viewable{can_be_split_into outer inner delta})
-  (v:t_of outer)
-  : Ghost (t_of inner)
-          (requires True)
-         (ensures fun v' -> (forall (h:hheap (fp_of outer)).
-           (assume (interp (fp_of inner) h);
-           (sel_of outer h) == v ==> (sel_of inner h) == v')))
-
-assume val right_sel
-  (outer inner:viewable)
-  (delta:viewable{can_be_split_into outer inner delta})
-  (v:t_of outer)
-  : Ghost (t_of delta)
-          (requires True)
-         (ensures fun v' -> (forall (h:hheap (fp_of outer)).
-           (assume (interp (fp_of delta) h);
-           (sel_of outer h) == v ==> (sel_of delta h) == v')))
-
-(** A shortcut for the normalization. We need to reduce all our recursive functions **)
-unfold
-let normal (#a:Type) (x:a) =
-  norm [delta_only [`%sel_of; `%t_of; `%fp_of;
-                    `%incorrect_left_sel; `%incorrect_right_sel;
-                    `%fst; `%snd]; iota; zeta] x
-
 effect Steel
   (a: Type)
-  (res0: viewable)
-  (res1: a -> viewable)
-  (pre: (t_of res0) -> prop)
-  (post: (t_of res0) -> (x:a) -> (t_of (res1 x)) -> prop)
+  (res0: hprop)
+  (res1: a -> hprop)
+  (pre: mem -> prop)
+  (post: mem -> a -> mem -> prop)
 = ST
   a
   (fun h0 ->
-    interp (fp_of res0) (heap_of_mem h0) /\
-    pre (normal (sel_of res0 (heap_of_mem h0))))
+    interp res0 (heap_of_mem h0) /\
+    pre h0)
   (fun h0 x h1 ->
-    interp (fp_of res0) (heap_of_mem h0) /\
-    pre (normal (sel_of res0 (heap_of_mem h0))) /\
-    interp (fp_of (res1 x)) (heap_of_mem h1) /\
-    post (normal (sel_of res0 (heap_of_mem h0)))
-         x
-         (normal (sel_of (res1 x) (heap_of_mem h1)))
+    interp res0 (heap_of_mem h0) /\
+    pre h0 /\
+    interp (res1 x) (heap_of_mem h1) /\
+    post h0 x h1
   )
 
-(** We underspecify get: It returns a heap about which we only know that
-    the resource invariant is satisfied, and that the views of the resouce
-    correspond to the ones we would compute from this heap **)
-assume val get (r:viewable)
-  :Steel (hheap (fp_of r)) (r) (fun _ -> r)
+assume val get (r:hprop)
+  :Steel (hmem r) (r) (fun _ -> r)
              (requires (fun m -> True))
-             (ensures (fun m0 x m1 -> m0 == m1 /\
-               m0 == normal (sel_of r x)))
+             (ensures (fun m0 x m1 -> m0 == x /\ m1 == m0))
 
-(*
-
-assume val put (r_init r_out:viewable) (m:hmem r_out.fp)
+assume val put (r_init r_out:hprop) (m:hmem r_out)
   :Steel unit (r_init) (fun _ -> r_out)
              (requires fun m -> True)
-             (ensures (fun _ _ m1 ->
-               affine_star r_out.fp (locks_invariant m) (heap_of_mem m);
-               m1 == r_out.sel (heap_of_mem m)))
-*)
+             (ensures (fun _ _ m1 -> m1 == m))
 
-(** A few lemmas to cast between the different pointer hprops **)
 let interp_perm_to_ptr (#a:Type) (p:permission) (r:ref a) (h:heap)
   : Lemma (requires interp (ptr_perm r p) h)
           (ensures interp (ptr r) h)
@@ -183,56 +72,38 @@ let pts_to_sel (#a:Type) (p:permission) (r:ref a) (v:a) (h:heap)
   = interp_pts_to_perm p r v h; interp_perm_to_ptr p r h;
     sel_lemma r p h;
     pts_to_injective r p v (sel r h) h
-(*
-let vptr_perm #a (r:ref a) (p:permission) = {
-  t = unit;
-  fp = ptr_perm r p;
-  sel = fun _ -> ()}
-
-let vptr #a (r:ref a) = {
-  t = a;
-  fp = ptr r;
-  sel = fun h -> sel r h}
-
-let vpts_to #a (r:ref a) (p:permission) (v:a) = {
-  t = a;
-  fp = pts_to r p v;
-  sel = fun _ -> v}
 
 val perm_to_ptr (#a:Type) (p:permission) (r:ref a) : Steel unit
-  (vptr_perm r p)
-  (fun _ -> vptr r)
+  (ptr_perm r p)
+  (fun _ -> ptr r)
   (fun _ -> True)
   (fun h0 _ h1 -> h0 == h1)
 
 let perm_to_ptr #a p r =
- admit();
- let h = get (vptr_perm r p) in
+ let h = get (ptr_perm r p) in
  interp_perm_to_ptr p r (heap_of_mem h)
 
 val pts_to_perm (#a:Type) (p:permission) (r:ref a) (v:a) : Steel unit
-  (vpts_to r p v)
-  (fun _ -> vptr_perm r p)
+  (pts_to r p v)
+  (fun _ -> ptr_perm r p)
   (fun _ -> True)
-  (fun h0 _ h1 -> True) // interp (ptr r) (heap_of_mem h1) /\ h0 == h1 /\ sel r (heap_of_mem h1) == v)
+  (fun h0 _ h1 -> interp (ptr r) (heap_of_mem h1) /\ h0 == h1 /\ sel r (heap_of_mem h1) == v)
 
 let pts_to_perm  #a p r v =
- admit();
- let h = get (vpts_to r p v) in
+ let h = get (pts_to r p v) in
  interp_pts_to_perm p r v (heap_of_mem h);
  interp_perm_to_ptr p r (heap_of_mem h);
  pts_to_sel p r v (heap_of_mem h)
 
 val ptr_read (#a:Type) (r:ref a) : Steel a
-  (vptr_perm r full_permission)
-  (fun v -> vpts_to r full_permission v)
+  (ptr_perm r full_permission)
+  (fun v -> pts_to r full_permission v)
   (fun _ -> True)
   (fun _ _ _ -> True)
 
 let ptr_read #a r =
- admit();
  perm_to_ptr full_permission r;
- let h = get (vptr r) in
+ let h = get (ptr r) in
  let v = sel r (heap_of_mem h) in
  sel_lemma r full_permission (heap_of_mem h);
  v
@@ -248,121 +119,68 @@ let ptr_update #a r v =
   let h = get (ptr_perm r full_permission) in
   let (| _, h' |) = upd r v h in
   put (ptr_perm r full_permission) (pts_to r full_permission v) h'
-*)
 
-(** Shortcut for a pointer with full permission **)
 let fptr (#a:Type) (r:ref a) : hprop = ptr_perm r full_permission
 
 let fsel (#a:Type) (r:ref a) (h:hheap (fptr r)) : a =
   interp_perm_to_ptr full_permission r h;
   sel r h
 
-(** The actual hprop with view for a pointer. Its view has the same type as the pointer **)
-let vptr (#a:Type) (r:ref a) : viewable = VUnit
-  ({ t = a;
-    fp = fptr r;
-    sel = fun h -> fsel r h })
-
 val fread (#a:Type) (r:ref a) : Steel a
-  (vptr r) (fun _ -> vptr r)
+  (fptr r) (fun _ -> fptr r)
   (requires fun _ -> True)
-  (ensures fun m0 v m1 -> m0 == m1 /\ m1 == v)
+  // TODO: Why is this assume needed?
+  (ensures fun _ v m1 -> assume (interp (fptr r) (heap_of_mem m1)); fsel r (heap_of_mem m1) == v)
 
-(** TODO: Reimplement this **)
-let fread #a r = admit()
-  // let v = ptr_read #a r in
-  // pts_to_perm full_permission r v;
-  // v
+let fread #a r =
+  let v = ptr_read #a r in
+  pts_to_perm full_permission r v;
+  v
 
 val fupd (#a:Type) (r:ref a) (v:a) : Steel unit
-  (vptr r) (fun _ -> vptr r)
+  (fptr r) (fun _ -> fptr r)
   (requires fun _ -> True)
-  (ensures fun _ _ m1 -> m1 == v)
+  // TODO: Why is this assume needed?
+  (ensures fun _ _ m1 -> assume (interp (fptr r) (heap_of_mem m1)); fsel r (heap_of_mem m1) == v)
 
-(** TODO: Reimplement this **)
-let fupd #a r v = admit()
-  // ptr_update r v;
-  // pts_to_perm full_permission r v
+let fupd #a r v =
+  ptr_update r v;
+  pts_to_perm full_permission r v
 
-(** A more convenient notation for VStar **)
-unfold
-let (<*>) (p q:viewable) : viewable = VStar p q
-
-(** For test purposes, assume that outer is a star.
-    Remove once left/right_sel are done correctly through tactics **)
 assume
 val frame
-  (outer:viewable{VStar? outer})
-  (#inner0:viewable)
+  (outer0:hprop)
+  (#inner0:hprop)
   (#a:Type)
-  (#inner1:a -> viewable)
-  (#delta:viewable{can_be_split_into outer inner0 delta})
-  (#pre:t_of inner0 -> prop)
-  (#post:t_of inner0 -> (x:a) -> t_of (inner1 x) -> prop)
+  (#inner1:a -> hprop)
+  (#[resolve_frame()]
+    delta:hprop{
+      FStar.Tactics.with_tactic
+      reprove_frame
+      (can_be_split_into outer0 inner0 delta /\ True)})
+  (#pre:mem -> prop)
+  (#post:mem -> a -> mem -> prop)
   ($f:unit -> Steel a inner0 inner1 pre post)
-  : Steel a
-          outer
-          (* Observe that we do not need to use tactics for the postresource here. *)
-          (fun v -> (inner1 v) <*> delta)
-          (* We should satisfy the precondition of the framed function, using only the views
-              of inner0 *)
-          (fun v -> pre (normal (incorrect_left_sel outer inner0 delta v)))
-          (* fst v1 is here the view of inner1, snd v1 the view of delta after execution
-              by definition of sel_of *)
-          (fun v0 x v1 ->
-            post (normal (incorrect_left_sel outer inner0 delta v0)) x (normal (fst v1)) /\
-           (normal (incorrect_right_sel outer inner0 delta v0)) == normal (snd v1))
-
-#set-options "--max_fuel 1 --max_ifuel 0"
-
-(** A few tests of framing and normalization. An interesting observation is that we
-    only need a fuel of 1 to obtain egalities on "atomic" resources inside delta.
-    TODO: Investigate why we still need a fuel of 1. It seems related to the deconstruction
-    of the tuples **)
+  : Steel a outer0 (fun v -> inner1 v `star` delta) pre post
 
 val test1 (#a:Type) (r1 r2:ref a) : Steel a
-  (vptr r1 <*> vptr r2)
-  (fun _ -> vptr r1 <*> vptr r2)
+  (ptr_perm r1 full_permission `star` ptr_perm r2 full_permission)
+  (fun v -> pts_to r1 full_permission v `star` ptr_perm r2 full_permission)
   (fun _ -> True)
-  (fun (ov1, ov2) v (v1, v2) -> ov1 == v1 /\ v == v1 /\ ov2 == v2)
+  (fun _ _ _ -> True)
 
 let test1 #a r1 r2 =
-  assume (can_be_split_into (vptr r1 <*> vptr r2) (vptr r1) (vptr r2));
-  frame (vptr r1 <*> vptr r2)
-        #_ #_ #_
-        #(vptr r2)
-        (fun () -> fread r1)
+  frame (ptr_perm r1 full_permission `star` ptr_perm r2 full_permission)
+//        #(ptr_perm r2 full_permission)
+        (fun () -> ptr_read r1)
 
-val test2 (#a:Type) (r1 r2 r3:ref a) : Steel a
-  (vptr r1 <*> vptr r2 <*> vptr r3)
-  (fun _ -> vptr r1 <*> (vptr r2 <*> vptr r3))
+val test2 (#a:Type) (r1 r2:ref a) : Steel a
+  (ptr_perm r1 full_permission `star` ptr_perm r2 full_permission)
+  (fun v -> pts_to r2 full_permission v `star` ptr_perm r1 full_permission)
   (fun _ -> True)
-  (fun ov x v ->
-    let ((ov1, ov2), ov3) = ov in
-    let (v1, (v2, v3)) = v in
-    v1 == x /\ v2 == ov2 /\ v3 == ov3)
+  (fun _ v _ -> True)
 
-let test2 #a r1 r2 r3 =
-  assume (can_be_split_into (vptr r1 <*> vptr r2 <*> vptr r3) (vptr r1) (vptr r2 <*> vptr r3));
-  frame (vptr r1 <*> vptr r2 <*> vptr r3)
-        #_ #_ #_
-        #(vptr r2 <*> vptr r3)
-        (fun () -> fread r1)
-
-
-val test3 (#a:Type) (r1 r2 r3 r4:ref a) : Steel a
-  (vptr r1 <*> vptr r2 <*> vptr r3 <*> vptr r4)
-  (fun _ -> vptr r1 <*> (vptr r2 <*> vptr r3 <*> vptr r4))
-  (fun _ -> True)
-  (fun ov x v ->
-    let (((ov1, ov2), ov3), ov4) = ov in
-    let (v1, ((v2, v3), v4)) = v in
-    v1 == x /\ v2 == ov2 /\ v3 == ov3 /\ v4 == ov4)
-
-let test3 #a r1 r2 r3 r4 =
-  assume (can_be_split_into (vptr r1 <*> vptr r2 <*> vptr r3 <*> vptr r4)
-         (vptr r1) (vptr r2 <*> vptr r3 <*> vptr r4));
-  frame (vptr r1 <*> vptr r2 <*> vptr r3 <*> vptr r4)
-        #_ #_ #_
-        #(vptr r2 <*> vptr r3 <*> vptr r4)
-        (fun () -> fread r1)
+let test2 #a r1 r2 =
+  let v = frame (ptr_perm r1 full_permission `star` ptr_perm r2 full_permission)
+        (fun () -> ptr_read r2) in
+  v
